\begin{enunciado}{\ejExtra}
  Sean $a$, $b \en \enteros$ tal que $(a:b) = 6$.
  Hallar todos los $d = (2a + b : 3a - 2b)$ y dar un ejemplo en cada caso.
\end{enunciado}

Conviene \textit{coprimizar}: $(a:b) = 6 \sisolosi
  \llaves{l}{
    a = 6A\\
    b = 6B
  }$ con $(A:B) \llamada{1}= 1$\\
$d =
  (2\cdot 6A + 6B : 3\cdot 6A - 2\cdot 6B) =
  (6\cdot( 2 \cdot A + B) : 6\cdot (3\cdot A - 2\cdot B)) =
  6 \cdot \ub{(2A + B : 3A - 2B)}{D}\\
  \to d \llamada{2}= 6 D \flecha{busco divisores}[comunes]
  \llave{l}{
    D \divideA 2A + B  \\
    D \divideA 3A - 2B \\
  } \flecha{operaciones}[$\dots$]
  \llave{l}{
    D \divideA 7B \\
    D \divideA 7A \\
  }\entonces
  D = (7A:7B) =7 \cdot (A:B) \llamada{1}= 7$  \\
Por lo tanto $D \en \divsetP{7}{1,7}$, pero yo quiero encontrar ejemplos de $a$ y $b$:\\
$\llamada{2}\to
  \llave{c}{
    d = 6 \cdot 7 = 42
    \llave{ll}{
      \text{Si:} & A = 2 \to a = 12 \\
                 & B = 3 \to b = 18 \\
      \multicolumn{2}{l}{(7:0)\entonces D = 7 \to d = (42:0) = \ub{42}{6\cdot D}}
    } \\

    \magenta{\o}                              \\
    d = 6 \cdot 1 = 6
    \llave{ll}{
      \text{Si:} & A = 0 \to a = 0 \\
                 & B = 1 \to b = 6 \\
      \multicolumn{2}{l}{(1:-2) \entonces D = 1 \to d = (6:-12) = \ub{6}{6\cdot D}}
    }
  }$
